mark-and-sweep/spec/GC.Spec.ChunkedMarkBounded.CountStep.fsti
@@ -1,0 +1,26 @@
+module GC.Spec.ChunkedMarkBounded.CountStep
+
+module Seq = FStar.Seq
+
+open GC.Spec.Base
+
+module MH = GC.Spec.MajorHeap
+module BDefs = GC.Spec.ChunkedMarkBounded.Defs
+module BPres = GC.Spec.ChunkedMarkBounded.Preservation
+
+val chunked_mark_step_bounded_decreases_count
+  (mh: MH.major_heap)
+  (st: Seq.seq obj_addr)
+  (cap: nat)
+  : Lemma
+      (requires
+        Seq.length st > 0 /\
+        MH.well_formed_major_heap mh /\
+        BPres.chunked_mark_step_bounded_preservation_ready mh st cap /\
+        Seq.mem (Seq.head st) (MH.major_objects mh) /\
+        BDefs.chunked_is_gray mh (Seq.head st))
+      (ensures
+        (let (mh', _) = BDefs.chunked_mark_step_bounded mh st cap in
+         BDefs.chunked_count_non_black mh' <
+         BDefs.chunked_count_non_black mh))
+
